@base <http://n2t.net/ark:/99152/p0v> .
@prefix rdfs: <http://www.w3.org/2000/01/rdf-schema#> .
@prefix owl: <http://www.w3.org/2002/07/owl#> .
@prefix time: <http://www.w3.org/2006/time#> .
@prefix xsd: <http://www.w3.org/2001/XMLSchema#> .
@prefix prov: <http://www.w3.org/ns/prov#> .

<#spatialCoverageDescription> a owl:DatatypeProperty ;
    rdfs:comment "Free-text description of the spatial coverage of a resource."@en ;
    rdfs:isDefinedBy <> ;
    rdfs:label "spatial coverage description"@en ;
    rdfs:range xsd:string .

<#earliestYear> a owl:DatatypeProperty ;
    rdfs:comment "The earliest Gregorian year referred to in the description of a temporal interval."@en ;
    rdfs:isDefinedBy <> ;
    rdfs:label "earliest year"@en ;
    rdfs:domain time:DateTimeDescription ;
    rdfs:range xsd:gYear .

<#latestYear> a owl:DatatypeProperty ;
    rdfs:comment "The latest Gregorian year referred to in the description of a temporal interval."@en ;
    rdfs:isDefinedBy <> ;
    rdfs:label "latest year"@en ;
    rdfs:domain time:DateTimeDescription ;
    rdfs:range xsd:gYear .

time:DateTimeDescription
    rdfs:subClassOf [
        a owl:Restriction ;
        owl:maxCardinality "1"^^xsd:nonNegativeInteger ;
        owl:onProperty <#earliestYear>
    ], [
        a owl:Restriction ;
        owl:maxCardinality "1"^^xsd:nonNegativeInteger ;
        owl:onProperty <#latestYear>
    ] .

<#submitted> a prov:Role ;
    rdfs:comment "The role played by the agent responsible for submitting a patch."@en ;
    rdfs:isDefinedBy <> ;
    rdfs:label "submitted"@en .

<#updated> a prov:Role ;
    rdfs:comment "The role played by the agent responsible for updating a patch."@en ;
    rdfs:isDefinedBy <> ;
    rdfs:label "updated"@en .

<#merged> a prov:Role ;
    rdfs:comment "The role played by the agent responsible for merging a patch."@en ;
    rdfs:isDefinedBy <> ;
    rdfs:label "merged"@en .

