@base <http://n2t.net/ark:/99152/> .

@prefix periodo: <p0v#> .

@prefix rdfs: <http://www.w3.org/2000/01/rdf-schema#> .
@prefix owl: <http://www.w3.org/2002/07/owl#> .
@prefix time: <http://www.w3.org/2006/time#> .
@prefix xsd: <http://www.w3.org/2001/XMLSchema#> .

periodo:spatialCoverageDescription a owl:DatatypeProperty ;
    rdfs:comment "Free-text description of the spatial coverage of a resource."@en ;
    rdfs:isDefinedBy <http://n2t.net/ark:/99152/p0v> ;
    rdfs:label "spatial coverage description"@en ;
    rdfs:range xsd:string .

periodo:earliestYear a owl:DatatypeProperty ;
    rdfs:comment "The earliest Gregorian year referred to in the description of a temporal interval."@en ;
    rdfs:isDefinedBy <http://n2t.net/ark:/99152/p0v> ;
    rdfs:label "earliest year"@en ;
    rdfs:domain time:DateTimeDescription ;
    rdfs:range xsd:gYear .

periodo:latestYear a owl:DatatypeProperty ;
    rdfs:comment "The latest Gregorian year referred to in the description of a temporal interval."@en ;
    rdfs:isDefinedBy <http://n2t.net/ark:/99152/p0v> ;
    rdfs:label "latest year"@en ;
    rdfs:domain time:DateTimeDescription ;
    rdfs:range xsd:gYear .

time:DateTimeDescription
    rdfs:subClassOf [
        a owl:Restriction ;
        owl:maxCardinality "1"^^xsd:nonNegativeInteger ;
        owl:onProperty periodo:earliestYear
    ], [
        a owl:Restriction ;
        owl:maxCardinality "1"^^xsd:nonNegativeInteger ;
        owl:onProperty periodo:latestYear
    ] .
